update with adam's PRF proof + comment on first half of it

src/FCF/RndInList.v.d
@@ -1,1 +1,1 @@
-RndInList.vo RndInList.glob RndInList.v.beautified: RndInList.v ./FCF.vo
+RndInList.vo RndInList.glob RndInList.v.beautified: RndInList.v ./FCF.vo ./CompFold.vo
